src/lowparse/LowParse.Low.Int.fst
@@ -12,16 +12,16 @@ module HS = FStar.HyperStack
 module B = LowStar.Buffer
 
 inline_for_extraction
-let parse32_u8 =
-  leaf_reader_ext Aux.parse32_u8 parse_u8 (fun x -> Unique.parse_u8_unique x)
+let read_u8 =
+  leaf_reader_ext Aux.read_u8 parse_u8 (fun x -> Unique.parse_u8_unique x)
 
 inline_for_extraction
-let parse32_u16 =
-  leaf_reader_ext Aux.parse32_u16 parse_u16 (fun x -> Unique.parse_u16_unique x)
+let read_u16 =
+  leaf_reader_ext Aux.read_u16 parse_u16 (fun x -> Unique.parse_u16_unique x)
 
 inline_for_extraction
-let parse32_u32 =
-  leaf_reader_ext Aux.parse32_u32 parse_u32 (fun x -> Unique.parse_u32_unique x)
+let read_u32 =
+  leaf_reader_ext Aux.read_u32 parse_u32 (fun x -> Unique.parse_u32_unique x)
 
 inline_for_extraction
 let serialize32_u8 : serializer32 serialize_u8 = fun v b ->
@@ -38,8 +38,8 @@ let serialize32_u32 : serializer32 serialize_u32 = fun v b ->
   [@inline_let] let _ = Unique.serialize_u32_unique v in
   Aux.serialize32_u32 v b
 
-let emit_u8 = leaf_writer_strong_of_serializer32 serialize32_u8 ()
+let write_u8 = leaf_writer_strong_of_serializer32 serialize32_u8 ()
 
-let emit_u16 = leaf_writer_strong_of_serializer32 serialize32_u16 ()
+let write_u16 = leaf_writer_strong_of_serializer32 serialize32_u16 ()
 
-let emit_u32 = leaf_writer_strong_of_serializer32 serialize32_u32 ()
+let write_u32 = leaf_writer_strong_of_serializer32 serialize32_u32 ()
